\documentclass[12pt, a4j]{jsarticle}
\usepackage[%
top    = 30truemm,%
bottom = 30truemm,%
left   = 25truemm,%
right  = 25truemm]{geometry}
\usepackage{amsmath,amssymb,amsthm}
\usepackage{bm,braket,ascmac,enumitem}
\usepackage{mathtools}
\mathtoolsset{showonlyrefs=true}


\newcommand{\p}{\partial}
\renewcommand{\Re}{\mathrm{Re}}


\begin{document}

基礎方程式:
\begin{gather}
    \p_{t} \bm{u} 
    + \bm{u} \cdot \nabla \bm{u}
    = - \nabla P 
      - \dfrac{1}{\Re_{0}} (\bm{u} - U_{y} \hat{\bm{y}})
      + \dfrac{1}{\Re} \nabla^{2} \bm{u}
      + \sin{(n y)} \hat{\bm{x}},
    \\
    \nabla \cdot \bm{u}
    = 0,
    \\
    \bm{U}
    = \dfrac{a}{4 \pi^{2}} \int dxdy \bm{u}
    = (0, U_{y})
    \quad : \text{const.}
\end{gather}

新しい変数:
\begin{equation}
    \bm{v} 
    = \bm{u} - \bm{U}
    = \nabla \times (\psi \hat{\bm{z}})
    = (\p_{y} \psi) \hat{\bm{x}}
      + (- \p_{x} \psi) \hat{\bm{y}}
\end{equation}

変換した基礎方程式:
\begin{gather}
    \p_{t} \bm{v} 
    + \bm{v} \cdot \nabla \bm{v}
    + \bm{U} \cdot \nabla \bm{v}
    = - \nabla P 
      - \dfrac{1}{\Re_{0}} \bm{v}
      + \dfrac{1}{\Re} \nabla^{2} \bm{v}
      + \sin{(n y)} \hat{\bm{x}},
    \\
    \nabla \cdot \bm{v}
    = 0,
    \\
    \dfrac{a}{4 \pi^{2}} \int dxdy \bm{v}
    = 0
\end{gather}

$\nabla \times$ を掛けたい:
\begin{gather}
    \nabla \times \bm{v}
    = \nabla \times \nabla \times (\psi \hat{\bm{z}})
    = \nabla (\nabla \cdot \psi \hat{\bm{z}})
      - \nabla^{2} (\psi \hat{\bm{z}})
    = (- \nabla^{2} \psi) \hat{\bm{z}}
    \\
    \nabla \times (\bm{v} \cdot \nabla \bm{v})
    = J(\psi, \nabla^{2} \psi) \hat{\bm{z}},
    \\
    \nabla \times (\bm{U} \cdot \nabla \bm{v})
    = \bm{U} \cdot \nabla (\nabla \times \bm{v})
    = (- U_{y} \p_{y} \nabla^{2} \psi) \hat{\bm{z}}
\end{gather}
ただし
\begin{equation}
    J(a, b)
    = (\p_{x} a) (\p_{y} b) - (\p_{y} a) (\p_{x} b)
\end{equation}

基礎方程式に $\nabla \times$ を掛ける:
\begin{equation}
    - \p_{t} \nabla^{2} \psi
    + J(\psi, \nabla^{2} \psi)
    - U_{y} \p_{y} \nabla^{2} \psi
    = \dfrac{1}{\Re_{0}} \nabla^{2} \psi
      - \dfrac{1}{\Re} \nabla^{2} \nabla^{2} \psi
      - n \cos{(n y)}
\end{equation}
整理:
\begin{align}
    \p_{t} \nabla^{2} \psi
    &= n \cos{(n y)}
       - \dfrac{1}{\Re_{0}} \nabla^{2} \psi
       - U_{y} \p_{y} \nabla^{2} \psi
       + \dfrac{1}{\Re} \nabla^{2} \nabla^{2} \psi \\
    &\hphantom{{}={}}
       + J(\psi, \nabla^{2} \psi)
\end{align}
$\omega
 = ( - \nabla^{2} \psi ) \cdot \hat{\bm{z}}
 = ( \nabla \times \bm{v} ) \cdot \hat{\bm{z}}$
とおいて整理:
\begin{align}
    \p_{t} \omega
    &= - n \cos{(n y)}
       - \dfrac{1}{\Re_{0}} \omega
       - U_{y} \p_{y} \omega
       + \dfrac{1}{\Re} \nabla^{2} \omega \\
    &\hphantom{{}={}}
       + J(\psi, \omega)
\end{align}


線形部分 $+$ cos 部分:
\begin{equation}
    \p_{t} \omega
    = - n \cos{(n y)}
      - \dfrac{1}{\Re_{0}} \omega
      - U_{y} \p_{y} \omega
      + \dfrac{1}{\Re} \nabla^{2} \omega
\end{equation}
Fourier 変換 $F[\omega](k, \ell)$:
\begin{equation}
    \p_{t} F[\omega]
    = - F[n \cos{(n y)}]
      - \dfrac{1}{\Re_{0}} F[\omega]
      - i \ell U_{y} F[\omega]
      - \dfrac{1}{\Re} (k^{2} + \ell^{2}) F[\omega]
\end{equation}
整理:
\begin{gather}
    \p_{t} \{ F[\omega] e(t) \} 
    = - F[n \cos{(n y)}] e(t),
    \\
    e(t) = \exp{(t \alpha)},
    \\
    \alpha
    = \dfrac{1}{\Re_{0}}
      + i \ell U_{y}
      + \dfrac{1}{\Re} (k^{2} + \ell^{2})
\end{gather}
積分:
\begin{align}
    F[\omega](t)
    &= F[\omega](t_{0}) e(- t + t_{0})
       - e(- t) \int_{t_{0}}^{t} F[n \cos{(n y)}] e(s) d s
    \\
    &= F[\omega](t_{0}) e(- t + t_{0})
       - F[n \cos{(n y)}]
         \cdot \dfrac{1 - e(- t + t_{0})}{\alpha}
    \\
    &= \left(
           F[\omega](t_{0})
           + \dfrac{F[ n \cos{(n y)} ]}{\alpha}
       \right) e(- t + t_{0})
       - \dfrac{F[ n \cos{(n y)} ]}{\alpha}
\end{align}



\end{document}